update correctness proof

pregel-graph-coloring.dfy
@@ -20,10 +20,17 @@ class PregelGraphColoring
 		requires valid1(vAttr) && valid2(sent) && valid2(msg)
 		requires valid0(src) && valid0(dst)
 		modifies msg, sent
+		ensures sent[src, dst] ==> vAttr[src] == vAttr[dst];
+		ensures !sent[src, dst] ==> vAttr[src] != vAttr[dst];
 	{
-		if vAttr[src] != vAttr[dst] {
-			msg[src, dst] := true;
-			sent[src, dst] := true;
+		if vAttr[src] == vAttr[dst] {
+			sent[src,dst] := true;
+			sent[dst,src] := true;
+			msg[src,dst] := true;
+			msg[dst,src] := true;
+		} else {
+			sent[src,dst] := false;
+			sent[dst,src] := false;
 		}
 	}
 
@@ -45,13 +52,45 @@ class PregelGraphColoring
 	 * Correctness assertion
 	 ***********************/
 
-	predicate Validated()
+
+	function method correctlyColored(): bool
 		requires valid1(vAttr) && valid2(graph) && valid2(sent)
 		reads vAttr, this`graph, this`vAttr, this`sent, this`numVertices
 	{
-		// Adjacent vertices have different colors after the algorithm terminates.
-		forall i,j :: 0 <= i < vAttr.Length && 0 <= j < vAttr.Length ==> 
+		// adjacent vertices have different colors
+		forall i,j :: 0 <= i < numVertices && 0 <= j < numVertices ==> 
 			adjacent(i, j) ==> vAttr[i] != vAttr[j]
+	}
+	
+	method Validated(maxNumIterations: nat) returns (res: bool)
+		requires numVertices > 1 && maxNumIterations > 0
+		requires valid1(vAttr) && valid2(graph) && valid2(sent) && valid2(msg)
+		modifies this`numVertices, vAttr, msg, sent
+		ensures res
+	{
+		var numIterations := pregel(maxNumIterations);
+		res := numIterations <= maxNumIterations ==> correctlyColored();
+	}
+
+	function method noCollisions(): bool
+		requires valid1(vAttr) && valid2(graph) && valid2(sent)
+		reads vAttr, this`graph, this`vAttr, this`sent, this`numVertices
+	{
+		forall vid :: 0 <= vid < numVertices ==> noCollisionAt(vid)
+	}
+
+	function method noCollisionAt(src: VertexId): bool
+		requires valid0(src) && valid1(vAttr) && valid2(graph) && valid2(sent)
+		reads this`graph, this`sent, this`vAttr, this`numVertices, vAttr
+	{
+		forall dst :: 0 <= dst < numVertices ==> noCollisionBetween(src, dst)
+	}
+
+	function method noCollisionBetween(src: VertexId, dst: VertexId): bool
+		requires valid0(src) && valid0(dst) && valid1(vAttr) && valid2(graph) && valid2(sent)
+		reads this`graph, this`sent, this`vAttr, this`numVertices, vAttr
+	{
+		adjacent(src, dst) && !sent[src, dst] ==> vAttr[src] != vAttr[dst]
 	}
 
 	/******************
@@ -94,14 +133,15 @@ class PregelGraphColoring
 		requires valid1(vAttr) && valid2(graph) && valid2(sent)
 		reads vAttr, this`graph, this`vAttr, this`sent, this`numVertices
 	{
-		!active() ==> Validated()
+		!active() ==> correctlyColored()
 	}
 
-	method pregel(maxNumIterations: nat)
-		requires numVertices > 1
+	method pregel(maxNumIterations: nat) returns (numIterations: nat)
+		requires numVertices > 1 && maxNumIterations > 0
 		requires valid1(vAttr) && valid2(graph) && valid2(sent) && valid2(msg)
 		modifies vAttr, msg, sent
-		ensures inv()
+		ensures numIterations <= maxNumIterations ==> correctlyColored()
+		//ensures inv()
 	{
 		var vid := 0;
 		while vid < numVertices
@@ -110,12 +150,16 @@ class PregelGraphColoring
 			vid := vid + 1;
 		}
 		sent[0,0] := true;
-		var numIterations := 0;
+		numIterations := 0;
 
-		while active() && numIterations <= maxNumIterations
-			//TODO: Prove invariant inv()
+		witness_for_existence(); assert active();
+
+		while (exists i, j :: 0 <= i < numVertices && 0 <= j < numVertices && sent[i,j]) && numIterations <= maxNumIterations
+		//while active() && numIterations <= maxNumIterations
+			//invariant inv()
+			//invariant !active() ==> 1==0
+			invariant !(exists i, j :: 0 <= i < numVertices && 0 <= j < numVertices && sent[i,j]) ==> noCollisions()
 		{
-			numIterations := numIterations + 1;
 			forall i,j | (0 <= i < numVertices && 0 <= j < numVertices)
 			{
 				sent[i,j] := false;
@@ -123,20 +167,30 @@ class PregelGraphColoring
 			var src := 0;
 			// invoke SendMessage on each edage
 			while src < numVertices
+				invariant src <= numVertices
+				invariant forall vid :: 0 <= vid < src ==> noCollisionAt(vid)
+				invariant numIterations > maxNumIterations ==> noCollisions()
 			{
 				var dst := 0;
 				while dst < numVertices
+					invariant dst <= numVertices
+					invariant forall vid :: 0 <= vid < dst ==> noCollisionBetween(src, vid);
+					invariant forall vid :: 0 <= vid < src ==> noCollisionAt(vid)
 				{
 					if adjacent(src, dst)
 					{
 						SendMessage(src, dst, graph[src,dst]);
 					}
+					assert noCollisionBetween(src, dst);
 					dst := dst + 1;
 				}
+				assert noCollisionAt(src);
 				src := src + 1;
 			}
-			// Has there at least one message been sent?
-			if active()
+			assert noCollisions();
+			//assert exists i, j :: 0 <= i < numVertices && 0 <= j < numVertices && sent[i,j]; // WRONGLY VERIFIED
+			//assert inv();
+			if exists i, j :: 0 <= i < numVertices && 0 <= j < numVertices && sent[i,j]
 			{
 				var dst := 0;
 				while dst < numVertices
@@ -169,7 +223,25 @@ class PregelGraphColoring
 					}
 					dst := dst + 1;
 				}
+				assert active();
 			}
+			assert !(exists i, j :: 0 <= i < numVertices && 0 <= j < numVertices && sent[i,j]) ==> noCollisions();
+			numIterations := numIterations + 1;
 		}
+
+		//assert numIterations <= maxNumIterations ==> forall i, j :: 0 <= i < numVertices && 0 <= j < numVertices ==> !sent[i,j];
+		assert numIterations <= maxNumIterations ==> !active();
+		
+		assert numIterations <= maxNumIterations ==> noCollisions();
+
+		//assert (forall i, j :: 0 <= i < numVertices && 0 <= j < numVertices ==> !sent[i,j]) && noCollisions() ==> correctlyColored();
+		assert !active() && noCollisions() ==> correctlyColored();
+
+		assert numIterations <= maxNumIterations ==> correctlyColored();
 	}
+
+	lemma witness_for_existence()
+		requires valid2(sent) && numVertices > 0 && sent[0,0]
+		ensures active()
+	{}
 }
